new/proof/github_com/tchajed/marshal.v
@@ -1,0 +1,12 @@
+Require Import New.generatedproof.github_com.tchajed.marshal.
+Require Import New.proof.proof_prelude.
+Require Import New.proof.github_com.goose_lang.std.
+
+Section heap.
+Context `{hG: heapGS Σ, !ffi_semantics _ _}.
+Context `{!goGlobalsGS Σ}.
+
+#[global]
+Program Instance : IsPkgInit marshal := ltac2:(build_pkg_init ()).
+
+End heap.
